Foundation/FirstOrder/Basic/Soundness.lean
@@ -12,55 +12,51 @@ namespace FirstOrder
 section sound
 open Semiformula
 
-variable {L : Language} {T : Theory L}
+variable {L : Language}
 
 namespace Derivation
 
-lemma sound (M : Type*) [s : Structure L M] [Nonempty M] [M ⊧ₘ* T] (ε : ℕ → M) {Γ : Sequent L} :
-    (T : Schema L) ⟹ Γ → ∃ φ ∈ Γ, Evalfm M ε φ
-  | axm (φ := φ) h => ⟨φ, by simp, by
-      have : ∃ σ ∈ T, ↑σ = φ := by simpa [Theory.toSchema] using h
-      rcases this with ⟨σ, hσ, rfl⟩
-      simpa using Theory.models M T hσ⟩
-  | axL r v => by
-    by_cases h : s.rel r (Semiterm.valm M ![] ε ∘ v)
+lemma sound {M : Type*} [s : Structure L M] [Nonempty M] (f : ℕ → M) {Γ : Sequent L} :
+    ⊢ᴷ Γ → ∃ φ ∈ Γ, φ.Evalf f
+  | identity r v => by
+    by_cases h : s.rel r (Semiterm.val ![] f ∘ v)
     · exact ⟨rel r v, by simp, h⟩
     · exact ⟨nrel r v, by simp, h⟩
   | verum => ⟨⊤, by simp⟩
   | or (Γ := Γ) (φ := φ) (ψ := ψ) d => by
-    have : Evalfm M ε φ ∨ Evalfm M ε ψ ∨ ∃ ψ ∈ Γ, Evalfm M ε ψ := by simpa using sound M ε d
+    have : Evalf f φ ∨ Evalf f ψ ∨ ∃ ψ ∈ Γ, Evalf f ψ := by simpa using sound f d
     rcases this with (hp | hq | ⟨r, hr, hhr⟩)
     · exact ⟨φ ⋎ ψ, by simp, by simp [hp]⟩
     · exact ⟨φ ⋎ ψ, by simp, by simp [hq]⟩
     · exact ⟨r, by simp [hr], hhr⟩
   | and (Γ := Γ) (φ := φ) (ψ := ψ) dp dq => by
-    have : Evalfm M ε φ ∨ ∃ r ∈ Γ, Evalfm M ε r := by simpa using sound M ε dp
+    have : Evalf f φ ∨ ∃ r ∈ Γ, Evalf f r := by simpa using sound f dp
     rcases this with (hp | ⟨r, hr, hhr⟩)
-    · have : Evalfm M ε ψ ∨ ∃ r ∈ Γ, Evalfm M ε r := by simpa using sound M ε dq
+    · have : Evalf f ψ ∨ ∃ r ∈ Γ, Evalf f r := by simpa using sound f dq
       rcases this with (hq | ⟨r, hr, hhr⟩)
       · exact ⟨φ ⋏ ψ, by simp, by simp [hp, hq]⟩
       · exact ⟨r, by simp [hr], hhr⟩
     · exact ⟨r, by simp [hr], hhr⟩
   | all (Γ := Γ) (φ := φ) d => by
-    have : (∀ a : M, Evalm M ![a] ε φ) ∨ ∃ ψ ∈ Γ, Evalfm M ε ψ := by
+    have : (∀ a : M, Eval ![a] f φ) ∨ ∃ ψ ∈ Γ, Evalf f ψ := by
       simpa [Rewriting.shifts, Matrix.vecConsLast_vecEmpty, forall_or_right]
-        using fun a : M => sound M (a :>ₙ ε) d
+        using fun a : M => sound (a :>ₙ f) d
     rcases this with (hp | ⟨ψ, hq, hhq⟩)
     · exact ⟨∀⁰ φ, by simp, hp⟩
     · exact ⟨ψ, by simp [hq], hhq⟩
-  | exs (Γ := Γ) (φ := φ) t d => by
-    have : Evalm M ![t.valm M ![] ε] ε φ ∨ ∃ φ ∈ Γ, Evalfm M ε φ := by
-      simpa [eval_substs, Matrix.constant_eq_singleton] using sound M ε d
+  | exs (Γ := Γ) (φ := φ) (t := t) d => by
+    have : Eval ![t.val ![] f] f φ ∨ ∃ φ ∈ Γ, Evalf f φ := by
+      simpa [eval_substs, Matrix.constant_eq_singleton] using sound f d
     rcases this with (hp | ⟨ψ, hq, hhq⟩)
-    · exact ⟨∃⁰ φ, by simp, t.valm M ![] ε, hp⟩
+    · exact ⟨∃⁰ φ, by simp, t.val ![] f, hp⟩
     · exact ⟨ψ, by simp [hq], hhq⟩
   | wk (Δ := Δ) (Γ := Γ) d ss => by
-    have : ∃ φ ∈ Δ, Evalfm M ε φ := sound M ε d
+    have : ∃ φ ∈ Δ, Evalf f φ := sound f d
     rcases this with ⟨φ, hp, h⟩
     exact ⟨φ, ss hp, h⟩
-  | cut (Γ := Γ) (φ := φ) d dn => by
-    have h : Evalfm M ε φ ∨ ∃ ψ ∈ Γ, Evalfm M ε ψ := by simpa using sound M ε d
-    have hn : ¬Evalfm M ε φ ∨ ∃ ψ ∈ Γ, Evalfm M ε ψ := by simpa using sound M ε dn
+  | cut (Γ := Γ) (Δ := Δ) (φ := φ) d dn => by
+    have h : Evalf f φ ∨ ∃ ψ ∈ Γ, Evalf f ψ := by simpa using sound f d
+    have hn : ¬Evalf f φ ∨ ∃ ψ ∈ Δ, Evalf f ψ := by simpa using sound f dn
     rcases h with (h | ⟨ψ, h, hq⟩)
     · rcases hn with (hn | ⟨ψ, hn, hq⟩)
       · contradiction
@@ -69,16 +65,32 @@ lemma sound (M : Type*) [s : Structure L M] [Nonempty M] [M ⊧ₘ* T] (ε : ℕ
 
 end Derivation
 
-theorem sound : T ⊢! σ → T ⊨[Struc.{v, u} L] σ := fun b s hT ↦ by
-  have : s.Dom ⊧ₘ* T := hT
-  have : Inhabited s.Dom := Classical.inhabited_of_nonempty s.nonempty
-  simpa using Derivation.sound s.Dom default b
+theorem Provable.sound {M : Type*} [s : Structure L M] [Nonempty M] {φ : Proposition L} (f : ℕ → M) :
+    𝐋𝐊¹ ⊢ φ → φ.Evalf f := fun b ↦ by simpa using Derivation.sound f b.get
 
-theorem sound! : T ⊢ σ → T ⊨[Struc.{v, u} L] σ := fun ⟨b⟩ ↦ sound b
+variable {𝔖 : Schema L}
 
-theorem smallSound : T ⊢! σ → T ⊨ σ := sound
+theorem Schema.sound_proposition {M : Type*} [s : Structure L M] [Nonempty M] :
+    𝔖 ⊢ φ → M↓[L] ⊧* 𝔖 → ∀ f : ℕ → M, φ.Evalf f := fun b H f ↦ by
+  rcases Schema.provable_iff.mp b with ⟨Γ, hΓ, ⟨b⟩⟩
+  have : φ.Evalf f ∨ ∃ ψ, ∼ψ ∈ Γ ∧ ψ.Evalf f := by simpa using b.sound f
+  rcases this with (h | ⟨ψ, hψ, h⟩)
+  · assumption
+  · have : ¬ψ.Evalf f := by
+      have := by simpa [models_iff] using H.models _ (φ := (∼ψ).univCl) (by grind only [Schema.mem_uniClosure])
+      exact this f
+    contradiction
 
-theorem smallSound! : T ⊢ σ → T ⊨ σ := sound!
+theorem Schema.sound_proposition' :
+    𝔖 ⊢ φ → (𝔖 : Theory L) ⊨[Struc.{v, u} L] φ.univCl := fun b s hS ↦ by
+  simpa [struc_models_iff_models (s := s), models_iff]
+    using Schema.sound_proposition b hS
+
+theorem Schema.sound_sentence {σ : Sentence L} :
+    𝔖 ⊢ ↑σ → (𝔖 : Theory L) ⊨[Struc.{v, u} L] σ := fun b ↦ by
+  simpa using Schema.sound_proposition' b
+
+theorem Schema.smallSound_sentence (σ : Sentence L) : 𝔖 ⊢ ↑σ → (𝔖 : Theory L) ⊨ σ := Schema.sound_sentence
 
 instance (T : Theory L) : Sound T (Semantics.models (Struc.{v, u} L) T) := ⟨sound!⟩
 
@@ -95,7 +107,7 @@ lemma consistent_of_model (T : Theory L) (M : Type*) [s : Structure L M] [Nonemp
 
 lemma unprovable_of_countermodel {M : Type*} [s : Structure L M] [Nonempty M] [hM : M ⊧ₘ* T]
     {σ} (c : ¬M ⊧ₘ σ) : T ⊬ σ := by
-  apply Sound.not_provable_of_countermodel (𝓜 := Semantics.models (Struc L) T) (𝓢 := T)
+  apply Sound.not_provable_of_countermodel (𝓜 := Semantics.models (Struc L) T) (𝔖 := T)
   intro h
   exact c (h hM)
 
